Lifting from Lang to MLang

theories/interop/lang_to_mlang.v
@@ -1,7 +1,7 @@
 From Coq Require Import ssreflect.
 From stdpp Require Import strings gmap.
 From melocoton.mlanguage Require Import mlanguage.
-From melocoton.interop Require Import linking.
+(* From melocoton.interop Require Import linking. *)
 From melocoton.language Require Import language.
 
 Section ToMlang.
@@ -10,37 +10,58 @@ Section ToMlang.
 
   Local Notation prog := (gmap string Λ.(func)).
   Local Notation expr_state := ((Λ.(expr) * Λ.(state)))%type.
-  Inductive head_step_mrel : prog -> expr_state -> (expr_state->Prop) -> Prop := 
-    wrap p e1 σ1 e2 σ2 (Y : _ → Prop) : Λ.(head_step) p e1 σ1 e2 σ2 [] → 
-    (forall e2' σ2', e2 = e2' ∧ σ2 = σ2' → Y (e2', σ2')) → head_step_mrel p (e1,σ1) Y.
 
-  Program Definition head_step (p : prog) : umrel (expr_state) :=
-    {| mrel := head_step_mrel p |}.
+  Inductive prim_step_mrel : prog -> expr_state -> (expr_state->Prop) -> Prop := 
+  | WrapStep p e1 σ1 e2 σ2 (X : _ → Prop) : 
+        prim_step p e1 σ1 e2 σ2 [] → 
+        (X (e2, σ2)) →
+      prim_step_mrel p (e1,σ1) X
+  | WrapUbStep p e1 σ1 X :
+        stuck_no_threads p e1 σ1 →
+      prim_step_mrel p (e1,σ1) X.
+
+  Program Definition prim_step (p : prog) : umrel (expr_state) :=
+    {| mrel := prim_step_mrel p |}.
   Next Obligation.
     intros p. intros [e1 σ1] X Y Hstep HXY. inversion Hstep; subst.
-    eapply (wrap p e1 σ1 e2 σ2); first done. intros ? ? (<- & <-).
-    apply HXY, H4. done.
+    - eapply (WrapStep p e1 σ1 e2 σ2); first done. apply HXY, H4.
+    - by eapply (WrapUbStep p e1 σ1).
   Qed.
 
+  Notation cont := Λ.(ectx).
+
+  Definition is_call (e : Λ.(expr)) (s : string) (vs : list val) (C : cont) : Prop := 
+    e = fill C (of_class Λ (ExprCall s vs)).
+
+  Axiom (XM : forall P , P ∨ ¬ P).
+
   Lemma language_mlanguage_mixin :
-    MlanguageMixin (val:=val) Λ.(of_class) Λ.(to_class) Λ.(empty_ectx) Λ.(comp_ectx) Λ.(fill)
-      Λ.(apply_func) head_step.
+    MlanguageMixin (val:=val) (of_val Λ) to_val is_call (fill) (Λ.(apply_func)) prim_step.
   Proof using.
-    constructor; try apply language_mixin.
-    - intros p v σ H Hstep. inversion Hstep; subst. eapply val_head_step. apply H3.
-    - intros p f vs σ X. split; intros H.
-      + inversion H; subst. destruct (call_head_step p f vs σ e2 σ2 []) as [HL HR].
-        destruct (HL H3) as (fn & Heq1 & Heq2 & Heq3 & Heq4). eexists fn, e2. repeat split; try congruence.
-        apply H5. repeat split; congruence.
-      + destruct H as (fn & e2 & Heq1 & Heq2 & HX).
-        destruct (call_head_step p f vs σ e2 σ []) as [HL HR].
-        eapply wrap. 1: apply HR; by eexists. intros ? ? ( <- & <- ). apply HX.
-    - intros p K' K_redec e1 e1_redex σ X Heq1 Heq2 Hstep. inversion Hstep; subst.
-      eapply step_by_val; try done. unfold to_val. destruct (to_class e1) as [[]|]; try congruence. exfalso. easy.
-    - intros p K e σ X H. inversion H; subst.
-      destruct (head_ctx_step_val p K e σ e2 σ2 [] H3) as [HL|[v Hv]].
-      + now left.
-      + right. exists v. unfold to_val in Hv. destruct (to_class e) as [[]|]; try congruence.
+    constructor.
+    - apply to_of_val.
+    - apply of_to_val.
+    - intros p v σ X H; inversion H; simplify_eq.
+      + by eapply val_prim_step.
+      + destruct H4 as [H4 _]. rewrite to_of_val in H4; done.
+    - intros p e f vs C σ X ->. split; intros H.
+      + inversion H; simplify_eq.
+        * apply prim_step_call_inv in H3 as (er&fn&HH1&HH2&->&->&_).
+          intros ? ? ? ?; simplify_eq; simplify_map_eq; congruence.
+        * destruct H4 as [Hv Hpr]. intros fn e2 HH1 HH2; exfalso; eapply Hpr. 1: exact nil.
+          eapply fill_prim_step, head_prim_step, call_head_step. by repeat eexists.
+      + destruct (p !! f) as [fn|] eqn:Heq1; first destruct (apply_func fn vs) as [e2|] eqn:Heq2.
+        * eapply WrapStep; last by eapply H.
+          eapply fill_prim_step, head_prim_step, call_head_step. by repeat eexists.
+        * eapply WrapUbStep. split; first apply to_val_fill_call.
+          intros e' σ' efs (er&fn'&HH1&HH2&->&->&_)%prim_step_call_inv; repeat simplify_eq. congruence.
+        * eapply WrapUbStep. split; first apply to_val_fill_call.
+          intros e' σ' efs (er&fn'&HH1&HH2&->&->&_)%prim_step_call_inv; repeat simplify_eq.
+    - intros e [v Hv] f vs C ->. rewrite to_val_fill_call in Hv; done.
+    - intros p e σ H.
+      destruct (XM (∃ e2 σ2, language.prim_step p e σ e2 σ2 [])) as [(e2&σ2&Hl)|Hr].
+      + eapply WrapStep; last done. exact Hl.
+      + eapply WrapUbStep. split; first done. intros ? ? ? ?. eapply Hr. by do 2 eexists.
   Qed.
 
   Definition lang_to_mlang : mlanguage val :=
@@ -48,11 +69,11 @@ Section ToMlang.
 
   Inductive lang_to_mlang_split_state : Λ.(state) → Λ.(state) → unit → Prop :=
     split_state_refl σ : lang_to_mlang_split_state σ σ ().
-
+(*
   Global Program Instance lang_to_mlang_linkable : linkable lang_to_mlang Λ.(state) := {
     linking.private_state := unit;
     linking.split_state := lang_to_mlang_split_state;
   }.
   Next Obligation. intros *. inversion 1; inversion 1; by simplify_eq. Qed.
-
+ *)
 End ToMlang.
